execution_invariants_s.thy
@@ -128,7 +128,7 @@ next
     thus ?case
       using state_wellFormed_combine_step step.IH by fastforce 
   next
-    case (beginAtomic C s ls f ls' t C' C'' vis vis' newTxns txns)
+    case (beginAtomic C s ls f ls' t C' C'' vis vis')
     then show ?case
       by blast 
   next
